Cpc/Proofs/Rules/Re_loop_star.lean
@@ -7,13 +7,13 @@ open Smtm
 set_option linter.unusedVariables false
 set_option maxHeartbeats 10000000
 
-theorem cmd_step_re_concat_star_subsume2_properties
+theorem cmd_step_re_loop_star_properties
     (M : SmtModel) (hM : model_total_typed M)
     (s : CState) (args : CArgList) (premises : CIndexList) :
-  cmdTranslationOk (CCmd.step CRule.re_concat_star_subsume2 args premises) ->
+  cmdTranslationOk (CCmd.step CRule.re_loop_star args premises) ->
   AllHaveBoolType (premiseTermList s premises) ->
-  __eo_typeof (__eo_cmd_step_proven s CRule.re_concat_star_subsume2 args premises) = Term.Bool ->
+  __eo_typeof (__eo_cmd_step_proven s CRule.re_loop_star args premises) = Term.Bool ->
   StepRuleProperties M (premiseTermList s premises)
-    (__eo_cmd_step_proven s CRule.re_concat_star_subsume2 args premises) :=
+    (__eo_cmd_step_proven s CRule.re_loop_star args premises) :=
 by
   sorry
